ulib/FStar.Monotonic.Heap.fst
@@ -77,12 +77,12 @@ abstract let sel (#a:Type) (#rel:preorder a) (h:heap) (r:mref a rel) :GTot a
     else r.init
 
 (* Update. *)
-abstract let upd_tot (#a:Type) (#rel:preorder a) (h:heap) (r:mref a rel{h `contains` r}) (x:a) :heap
+private abstract let upd_tot (#a:Type) (#rel:preorder a) (h:heap) (r:mref a rel{h `contains` r}) (x:a) :heap
   = { h with memory = (fun r' -> if r.addr = r'
 			      then Some (| a, (x , rel) |)
                               else h.memory r') }
 
-abstract let upd (#a:Type) (#rel:preorder a) (h:heap) (r:mref a rel) (x:a) :GTot heap
+abstract let upd (#a:Type) (#rel:preorder a) (h:heap) (r:mref a rel) (x:a{rel (sel h r) x}) :GTot heap
   = if FStar.StrongExcludedMiddle.strong_excluded_middle (h `contains` r)
     then upd_tot h r x
     else
@@ -118,7 +118,7 @@ let modifies (s:set nat) (h0:heap) (h1:heap) =
  * update of a well-typed reference
  *)
 private let lemma_upd_contains_test
-  (#a:Type) (#rel:preorder a) (h0:heap) (r:mref a rel) (x:a)
+  (#a:Type) (#rel:preorder a) (h0:heap) (r:mref a rel) (x:a{rel (sel h0 r) x})
   :Lemma (h0 `contains` r ==>
           (let h1 = upd h0 r x in
            (forall (b:Type) (rel':preorder b) (r':mref b rel'). addr_of r' <> addr_of r ==> sel h0 r' == sel h1 r') /\
@@ -134,7 +134,7 @@ private let lemma_upd_contains_test
  * in h0, r' is well-typed, but in h1 it's not
  *)
 private let lemma_upd_contains_not_necessarily_well_typed_test
-  (#a:Type) (#rel:preorder a) (h0:heap) (r:mref a rel) (x:a)
+  (#a:Type) (#rel:preorder a) (h0:heap) (r:mref a rel) (x:a{rel (sel h0 r) x})
   :Lemma ((~ (r `unused_in` h0)) ==>
           (let h1 = upd h0 r x in
 	   h1 `contains` r /\
@@ -147,7 +147,7 @@ private let lemma_upd_contains_not_necessarily_well_typed_test
  * update of an unused reference
  *)
 private let lemma_upd_unused_test
-  (#a:Type) (#rel:preorder a) (h0:heap) (r:mref a rel) (x:a)
+  (#a:Type) (#rel:preorder a) (h0:heap) (r:mref a rel) (x:a{rel (sel h0 r) x})
   :Lemma (r `unused_in` h0 ==>
           (let h1 = upd h0 r x in
 	   h1 `contains` r /\
@@ -178,7 +178,7 @@ private let lemma_free_mm_test (#a:Type) (#rel:preorder a) (h0:heap) (r:mref a r
 				   (r' `unused_in` h0 <==> r' `unused_in` h1)))))
   = ()
 
-private let lemma_upd_modifies_test (#a:Type) (#rel:preorder a) (h:heap) (r:mref a rel{h `contains` r \/ r `unused_in` h}) (x:a)
+private let lemma_upd_modifies_test (#a:Type) (#rel:preorder a) (h:heap) (r:mref a rel{h `contains` r \/ r `unused_in` h}) (x:a{rel (sel h r) x})
   :Lemma (modifies (Set.singleton (addr_of r)) h (upd h r x))
   = ()
 
@@ -248,14 +248,14 @@ let lemma_sel_same_addr (#a:Type) (#rel:preorder a) (h:heap) (r1:mref a rel) (r2
 	 [SMTPat (sel h r1); SMTPat (sel h r2)]
   = ()
 
-let sel_upd1 (#a:Type) (#rel:preorder a) (h:heap) (r:mref a rel) (x:a) (r':mref a rel)
+let sel_upd1 (#a:Type) (#rel:preorder a) (h:heap) (r:mref a rel) (x:a{rel (sel h r) x}) (r':mref a rel)
   :Lemma (requires (addr_of r = addr_of r'))
          (ensures  (sel (upd h r x) r' == x))
          [SMTPat (sel (upd h r x) r')]
 
   = ()
 
-let sel_upd2 (#a:Type) (#b:Type) (#rela:preorder a) (#relb:preorder b) (h:heap) (r1:mref a rela) (r2:mref b relb) (x:b)
+let sel_upd2 (#a:Type) (#b:Type) (#rela:preorder a) (#relb:preorder b) (h:heap) (r1:mref a rela) (r2:mref b relb) (x:b{relb (sel h r2) x})
   :Lemma (requires (addr_of r1 <> addr_of r2))
          (ensures  (sel (upd h r2 x) r1 == sel h r1))
 	 [SMTPat (sel (upd h r2 x) r1)]
@@ -276,7 +276,7 @@ let in_dom_emp (#a:Type) (#rel:preorder a) (r:mref a rel)
 	 [SMTPat (r `unused_in` emp)]
   = ()
 
-let upd_contains_a_well_typed (#a:Type) (#b:Type) (#rela:preorder a) (#relb:preorder b) (h:heap) (r:mref a rela) (x:a) (r':mref b relb)
+let upd_contains_a_well_typed (#a:Type) (#b:Type) (#rela:preorder a) (#relb:preorder b) (h:heap) (r:mref a rela) (x:a{rela (sel h r) x}) (r':mref b relb)
   :Lemma (requires True)
          (ensures  (((upd h r x) `contains` r) /\
 
@@ -298,7 +298,7 @@ val equal_extensional: h1:heap -> h2:heap
 		         [SMTPat (equal h1 h2)]
 let equal_extensional h1 h2 = ()
 
-let upd_upd_same_ref (#a:Type) (#rel:preorder a) (h:heap) (r:mref a rel) (x:a) (y:a)
+let upd_upd_same_ref (#a:Type) (#rel:preorder a) (h:heap) (r:mref a rel) (x:a{rel (sel h r) x}) (y:a{rel x y})
   :Lemma (requires True)
          (ensures  (upd (upd h r x) r y == upd h r y))
 	 [SMTPat (upd (upd h r x) r y)]
